theory/Utils/Dictionary.v
@@ -8,8 +8,9 @@ Arguments dict_elems {K V} _.
 
 Fixpoint lookup_falist {K V : Type} `{Ord K} (v : V) (k : K) (kvs : list (K * V)) :=
   match kvs with
-  | nil => v
-  | cons (k' , v') kvs' => match ord_dec k k' with
+  | [] => v
+  | (k' , v') :: kvs' =>
+    match ord_dec k k' with
     | Lt => v
     | Eq => v'
     | Gt => lookup_falist v k kvs'
@@ -18,54 +19,56 @@ Fixpoint lookup_falist {K V : Type} `{Ord K} (v : V) (k : K) (kvs : list (K * V)
 
 Fixpoint update_falist {K V : Type} `{Ord K} (k : K) (v : V) (kvs : list (K * V)) : list (K * V) :=
   match kvs with
-  | nil => [ (k , v) ]
-  | cons (k' , v') kvs' => match ord_dec k k' with
-      | Lt => (k , v) :: (k' , v') :: kvs'
-      | Eq => (k , v) :: kvs'
-      | Gt => (k' , v') :: update_falist k v kvs'
-      end
+  | [] => [ (k , v) ]
+  | (k' , v') :: kvs' =>
+    match ord_dec k k' with
+    | Lt => (k , v) :: (k' , v') :: kvs'
+    | Eq => (k , v) :: kvs'
+    | Gt => (k' , v') :: update_falist k v kvs'
+    end
   end.
 
-Definition lookup_dict {K V : Type} `{Ord K} (v : V) (k : K) (kvs : dict K V) := lookup_falist v k (dict_elems kvs).
+Definition lookup_dict {K V : Type} `{Ord K} (v : V) (k : K) (kvs : dict K V) := 
+  lookup_falist v k (dict_elems kvs).
 
 Definition update_dict {K V : Type} `{Ord K} (k : K) (v : V) (kvs : dict K V) : dict K V :=
   Dict (update_falist k v (dict_elems kvs)).
 
 Lemma lookup_update_diffid {K V} `{Ord K} : forall (k k' : K) (v v_def : V) m,
-      k <> k' ->
-      lookup_dict v_def k (update_dict k' v m) =
-        lookup_dict v_def k m.
-  Proof.
-    intros.
-    unfold lookup_dict.
-    unfold update_dict.
-    destruct m as [m]; simpl.
-    induction m as [|[k0 v0] tl]; simpl.
-    - destruct ord_dec eqn:id_cond; auto.
+  k <> k' ->
+  lookup_dict v_def k (update_dict k' v m) =
+  lookup_dict v_def k m.
+Proof.
+  intros.
+  unfold lookup_dict.
+  unfold update_dict.
+  destruct m as [m]; simpl.
+  induction m as [|[k0 v0] tl]; simpl.
+  - destruct ord_dec eqn:id_cond; auto.
+    apply ord_eq in id_cond; contradiction.
+  - destruct (ord_dec k' k0) eqn:id_cond; simpl.
+    + apply ord_eq in id_cond; subst.
+      destruct (ord_dec k k0) eqn:id_cond; auto.
       apply ord_eq in id_cond; contradiction.
-    - destruct (ord_dec k' k0) eqn:id_cond; simpl.
-      + apply ord_eq in id_cond; subst.
-        destruct (ord_dec k k0) eqn:id_cond; auto.
-        apply ord_eq in id_cond; contradiction.
-      + destruct (ord_dec k k') eqn:id_cond'.
-        * apply ord_eq in id_cond'; subst; contradiction.
-        * rewrite ord_lt_trans with (y := k'); auto.
-        * reflexivity.
-      + rewrite IHtl; auto.
+    + destruct (ord_dec k k') eqn:id_cond'.
+      * apply ord_eq in id_cond'; subst; contradiction.
+      * rewrite ord_lt_trans with (y := k'); auto.
+      * reflexivity.
+    + rewrite IHtl; auto.
 Qed.
 
 Lemma lookup_update_sameid {K V} `{Ord K} : forall (k : K) (v v_def : V) m, 
-      lookup_dict v_def k (update_dict k v m) = v.
+  lookup_dict v_def k (update_dict k v m) = v.
 Proof.
-    intros.
-    unfold lookup_dict.
-    unfold update_dict.
-    destruct m as [m]; simpl.
-    induction m as [|[k0 v0] tl]; simpl.
-    - rewrite ord_refl; auto.
-    - destruct (ord_dec k k0) eqn:id_cond; simpl.
-      + rewrite ord_refl; auto.
-      + rewrite ord_refl; auto.
-      + rewrite id_cond.
-        exact IHtl.
-  Qed.
+  intros.
+  unfold lookup_dict.
+  unfold update_dict.
+  destruct m as [m]; simpl.
+  induction m as [|[k0 v0] tl]; simpl.
+  - rewrite ord_refl; auto.
+  - destruct (ord_dec k k0) eqn:id_cond; simpl.
+    + rewrite ord_refl; auto.
+    + rewrite ord_refl; auto.
+    + rewrite id_cond.
+      exact IHtl.
+Qed.
